Day 9 wip

problems/9/Problem9.dfy
@@ -1,6 +1,237 @@
+include "../../parser/split.dfy"
+include "../../parser/parseInt.dfy"
 module Problem9 {
-    method problem9_1(input: string) returns (x: int) {
-        return 3;
+    import opened Split
+    import opened ParseInt
+    import opened Std.Collections.Seq
+
+    method parseInput(input: string) returns (data: seq<int>) 
+        ensures |data| > 0
+        ensures forall x :: x in data ==> x >= 0
+    {
+        var lines := splitOnBreak(input);
+        expect |lines| == 2;
+        data := Map(Integer, split(lines[0], ""));
+        expect |data| > 0;
+        expect forall x :: x in data ==> x >= 0;
+    }
+
+    function sum(x: seq<int>): int
+    {
+        if |x| == 0 then 0 else x[0] + sum(x[1..])
+    }
+
+    lemma sumConcat(x: seq<int>, y: seq<int>)
+        ensures sum(x + y) == sum(x) + sum(y)
+    {
+        if |x| == 0 {
+            assert x + y == y;
+            assert sum(x + y) == sum(y);
+        }else{
+            assert x == [x[0]] + x[1..];
+            assert x + y == [x[0]] + x[1..] + y;
+            // assert sum(x + y) == x[0] + sum(x[1..] + y);
+            sumConcat(x[1..], y);
+            assert sum(x) == x[0] + sum(x[1..]);
+            assert sum(x[1..] + y) == sum(x[1..]) + sum(y);
+            assert sum(x + y) == (x+y)[0] + sum((x+y)[1..]);
+            assert (x+y)[1..]   == x[1..] + y;
+            // assert sum(x + y) == sum(x) + sum(y);
+        }
+    }
+
+    lemma sumNatsNat(xs: seq<int>)
+        requires forall x :: x in xs ==> x >= 0
+        ensures 0 <= sum(xs)
+    {
+        if |xs| == 0 {
+            assert sum(xs) == 0;
+            assert 0 <= sum(xs);
+        }else{
+            assert xs == [xs[0]] + xs[1..];
+            assert xs[0] in xs;
+            assert forall x :: x in xs[1..] ==> x in xs;
+            sumNatsNat(xs[1..]);
+        }
+    }
+    lemma sumNats(xs: seq<int>, i: int)
+        requires forall x :: x in xs ==> x >= 0
+        requires 0 <= i <= |xs|
+        requires |xs| > 0
+        ensures sum(xs[..i]) <= sum(xs)
+    {
+        sumNatsNat(xs);
+        if i == 0 {
+            assert sum(xs[..i]) == 0;
+            // assert sum(xs) == xs[0];
+            assert forall x :: x in xs[..i] ==> x in xs;
+            assert sum(xs[..i]) <= sum(xs);
+        }else{
+            sumNats(xs, i-1);
+            assert xs[..i] == xs[..i-1] + [xs[i-1]];
+            sumConcat(xs[..i-1], [xs[i-1]]);
+            assert xs[i-1] in xs;
+            sumNatsNat([xs[i-1]]);
+            assert forall x :: x in xs[..i] ==> x in xs;
+            assert forall x :: x in xs[i..] ==> x in xs;
+            // assert sum(xs[..i]) == sum(xs[..i-1]) + xs[i];
+            assert sum(xs[..i-1]) <= sum(xs[..i]);
+            assert xs == xs[..i] + xs[i..];
+            sumNatsNat(xs[i..]);
+            sumConcat(xs[..i], xs[i..]);
+            assert sum(xs[..i]) <= sum(xs);
+        }
+    }
+    datatype File = File(id: int, start: nat, length: nat)
+    datatype Empty = Empty(start: nat, length: nat)
+    method ExpandDrive(data: seq<int>) returns (drive: array<int>, empty: seq<(nat, nat)>, files: seq<(int, nat, nat)>)
+        requires |data| > 0
+        requires forall x :: x in data ==> x >= 0
+        ensures fresh(drive)
+    {
+        var length := sum(data);
+        expect length > 0;
+        drive := new int[length];
+        empty := [];
+        files := [];
+        var x := 0;
+        var id := 0;
+        for i := 0 to |data|
+            invariant sum(data[..i]) == x
+            invariant 0 <= x <= length
+
+        {
+            sumNats(data, i+1);
+            if i % 2 == 0 {
+                expect data[i] > 0;
+                expect x < length;
+                assert data == data[..i] + [data[i]] + data[i+1..];
+                sumConcat(data[..i], [data[i]]);
+                sumConcat(data[..i]+[data[i]], data[i+1..]);
+
+                for j := 0 to data[i] 
+                {
+                    drive[x+j] := id;
+                }
+                assert data[..i+1] == data[..i] + [data[i]];
+                files := files + [(id, x as nat, data[i] as nat)];
+                sumConcat(data[..i], [data[i]]);
+                x := x + data[i];
+                id := id + 1;
+            }else{
+                if data[i] != 0 {
+                    assert data[i] in data;
+                    empty := empty + [(x as nat, data[i] as nat)];
+                    sumConcat(data[..i], [data[i]]);
+                    assert data[..i+1] == data[..i] + [data[i]];
+                    for j := 0 to data[i] 
+                    {
+                        drive[x+j] := -1;
+                    }
+                    x := x + data[i];
+                }else {
+                    sumConcat(data[..i], [data[i]]);
+                    assert data[..i+1] == data[..i] + [data[i]];
+                    x := x + data[i];
+                    assert x == sum(data[..i+1]);
+                }
+            }
+        }
+    }
+
+    method printDrive(drive: array<int>)
+    {
+        for i := 0 to drive.Length
+        {
+            if drive[i] != -1 {
+                print drive[i],",";
+            }else{
+                print ".";
+            }
+        }
+        print "\n";
+    }
+
+    method checksumDrive(drive: array<int>) returns (x: int)
+    {
+        x := 0;
+        for i := 0 to drive.Length
+        {
+            if drive[i] != -1 {
+                x := x + drive[i]*i;
+            }
+        }
+    }
+
+    method problem9_1(input: string) returns (x: int) 
+    {
+        var data := parseInput(input);
+        var drive, empty, files := ExpandDrive(data);
+        // printDrive(drive);
+        print |empty|, "\n";
+        print |files|, "\n";
+        while |empty| > 1 && |files| > 0
+            decreases |empty| + |files|
+        {
+            // printDrive(drive);
+            // print empty, " ", files, "\n";
+            var lastFile := files[|files|-1];
+            var firstEmpty := empty[0];
+            if lastFile.2 < firstEmpty.1 {
+                for i := 0 to lastFile.2
+                {
+                    expect 0 <= firstEmpty.0+i < drive.Length, "firstEmpty.0+i >= drive.Length: ";
+                    drive[firstEmpty.0+i] := lastFile.0;
+                    expect 0 <= lastFile.1+i < drive.Length, "lastFile.1+i >= drive.Length: ";
+                    drive[lastFile.1+i] := -1;
+                }
+                empty := [(firstEmpty.0+lastFile.2, firstEmpty.1-lastFile.2)]+empty[1..];
+                files := files[..|files|-1];
+                if empty[|empty|-1].0 < lastFile.1 {
+                    empty := empty + [(lastFile.1, lastFile.2)];
+                }else{
+                    if |empty| > 1 && empty[|empty|-2].0 + empty[|empty|-2].1 == lastFile.1 {
+                        empty := empty[..|empty|-2] + [(empty[|empty|-2].0, empty[|empty|-2].1 + lastFile.2 + empty[|empty|-1].1)];
+                    }else{
+                        empty := empty[..|empty|-1] + [(lastFile.1, lastFile.2 + empty[|empty|-1].1)];
+                    }
+                }
+            } else if lastFile.2 == firstEmpty.1 {
+                for i := 0 to lastFile.2
+                {
+                    expect 0 <= firstEmpty.0+i < drive.Length, "firstEmpty.0+i >= drive.Length: ";
+                    drive[firstEmpty.0+i] := lastFile.0;
+                    expect 0 <= lastFile.1+i < drive.Length, "lastFile.1+i >= drive.Length: ";
+                    drive[lastFile.1+i] := -1;
+                }
+
+                empty := empty[1..];
+                files := files[..|files|-1];
+                if empty[|empty|-1].0 < lastFile.1 {
+                    empty := empty + [(lastFile.1, lastFile.2)];
+                }else{
+                    if |empty| > 1 && empty[|empty|-2].0 + empty[|empty|-2].1 == lastFile.1 {
+                        empty := empty[..|empty|-2] + [(empty[|empty|-2].0, empty[|empty|-2].1 + lastFile.2 + empty[|empty|-1].1)];
+                    }else{
+                        empty := empty[..|empty|-1] + [(lastFile.1, lastFile.2 + empty[|empty|-1].1)];
+                    }
+                }
+            } else {
+                var newFile := (lastFile.0, lastFile.1, lastFile.2 - firstEmpty.1);
+                for i := 0 to firstEmpty.1
+                {
+                    expect 0 <= firstEmpty.0+i < drive.Length, "firstEmpty.0+i >= drive.Length: ";
+                    drive[firstEmpty.0+i] := lastFile.0;
+                    expect 0 <= lastFile.1+lastFile.2-(i+1) < drive.Length, "lastFile.1+lastFile.2-(i+1) >= drive.Length: ";
+                    drive[lastFile.1+lastFile.2-(i+1)] := -1;
+                }
+                files := files[..|files|-1] + [newFile];
+                empty := empty[1..];
+            }
+            // expect multiset(drive[..]) == multiset(old(drive)[..]);
+        }
+        // printDrive(drive);
+        x := checksumDrive(drive);
     }
 
     method problem9_2(input: string) returns (x: int) {
